Temporary commit to save work

src/Permutations/PermutationDefinitions.v
@@ -4,6 +4,7 @@ Require Import CoreData.ZXCore.
 (* FIXME: In QuantumLib *)
 Notation idn := (fun (k : nat) => k).
 
+(* TODO: Switch to 0 => k *)
 (* FIXME: In QuantumLib *)
 Fixpoint perm_inv n f : nat -> nat :=
   fun k => match n with
@@ -44,4 +45,24 @@ Fixpoint insertion_sort_list n f :=
   | 0 => []
   | S n' => let k := (perm_inv (S n') f n') in
       k :: insertion_sort_list n' (fswap f k n')
+  end.
+
+Fixpoint swap_list_spec l : bool :=
+  match l with 
+  | [] => true
+  | k :: ks => (k <? S (length ks)) && swap_list_spec ks
+  end.
+
+Fixpoint perm_of_swap_list l :=
+  match l with
+  | [] => idn
+  | k :: ks => let n := length ks in
+    (swap_perm k n (S n) ∘ (perm_of_swap_list ks))%prg
+  end.
+
+Fixpoint invperm_of_swap_list l :=
+  match l with 
+  | [] => idn
+  | k :: ks => let n := length ks in
+    ((invperm_of_swap_list ks) ∘ swap_perm k n (S n))%prg
   end.
